Completeness progress

Core/Linearizability.v
@@ -18,33 +18,39 @@ Definition KConc {T E} (spec : Spec T E) : Spec T E := overObj (spec :> idImpl).
 Definition Lin {T E} (spec' spec : Spec T E) :=
   specRefines spec' (KConc spec).
 
-Definition HBRw_ {T E} (evs evs' : Trace (ThreadEvent T E)) : Prop :=
-    exists h h' i i' m m',
-      i <> i' /\
-      evs = h ++ [(i, m); (i', m')] ++ h' /\
-      ((exists Ret e, m = @CallEv E Ret e) \/
-       (exists Ret e v, m' = @RetEv E Ret e v)) /\
-      evs' = h ++ [(i', m'); (i, m)] ++ h'.
+Variant HBRw_ {T E} : Trace (ThreadEvent T E) -> Trace (ThreadEvent T E) -> Prop :=
+| SwapCalls l r i j A (m : E A) B (n : E B) :
+    i <> j ->
+    HBRw_ (l ++ [(i, CallEv m); (j, CallEv n)] ++ r)
+          (l ++ [(j, CallEv n); (i, CallEv m)] ++ r)
+| SwapRets l r i j A (m : E A) v B (n : E B) w :
+    i <> j ->
+    HBRw_ (l ++ [(i, RetEv m v); (j, RetEv n w)] ++ r)
+          (l ++ [(j, RetEv n w); (i, RetEv m v)] ++ r)
+| DelayCall l r i j A (m : E A) B (n : E B) w :
+    i <> j ->
+    HBRw_ (l ++ [(i, CallEv m); (j, RetEv n w)] ++ r)
+          (l ++ [(j, RetEv n w); (i, CallEv m)] ++ r).
 
 Definition HBRw {T E} : (Trace (ThreadEvent T E)) -> (Trace (ThreadEvent T E)) -> Prop :=
-  clos_refl_trans (Trace (ThreadEvent T E)) HBRw_.
+  clos_refl_trans_1n (Trace (ThreadEvent T E)) HBRw_.
 
 Inductive AllRetEv {T E} : Trace (@ThreadEvent T E) -> Prop :=
 | NilAllRet : AllRetEv nil
 | ConsAllRet {Ret s i} {m : E Ret} {v : Ret} :
     AllRetEv s ->
-    AllRetEv (cons (i, RetEv m v) s).
+    AllRetEv ((i, RetEv m v) :: s).
 
 Inductive AllCallEv {T E} : Trace (ThreadEvent T E) -> Prop :=
 | NilAllCall : AllCallEv nil
 | ConsCall {Ret s i} {m : E Ret} :
     AllCallEv s ->
-    AllCallEv (cons (i, CallEv m) s).
+    AllCallEv ((i, CallEv m) :: s).
 
-Definition LinRw {T E} : 
+Definition LinRw {T E} :
   (Trace (ThreadEvent T E)) -> (Trace (ThreadEvent T E)) -> Prop :=
-  fun s t => exists sO sP, 
-    AllRetEv sP /\ AllCallEv sO /\
-    HBRw (s ++ sP) (t ++ sO).
+  fun s t => exists sC sR, 
+    AllRetEv sR /\ AllCallEv sC /\
+    HBRw (s ++ sR) (t ++ sC).
 
-Notation LinToSpec ρ V := (exists l, IsTraceOfSpec l V /\ LinRw ρ l). 
+Infix "~~>" := LinRw (at level 40).
