Core/WkPre.v
@@ -1,0 +1,29 @@
+From LHL.Core Require Import
+  Program
+  Traces
+  Logic
+  Specs.
+
+Section wp.
+
+Context
+  {T E F} {A : Type}
+  {VE : Spec T E} {VF : Spec T F}
+  (M : Impl E F) (i : Name T)
+  (m : F A) (Q : Post VE VF A).
+
+Definition wp : Prec VE VF :=
+  fun s ρs =>
+    forall p t v,
+      fst s i = Cont m (M A m) ->
+      InterSteps (spec:=VE) M s p t ->
+      fst t i = Cont m (Return v) ->
+      exists σs,
+        Q v s ρs t σs.
+
+Lemma wp_weakest {G : Relt VE VF} e :
+  w
+  Commit i G wp e Q.
+
+
+End wp.
